\section*{Exercise 1.16}

The whole process here depends on the computations for even and odd numbers.

\begin{equation}
	b^n = \left(b^2\right)^{n/2} = \left(b_{\text{new}}\right)^{n_{\text{new}}}
\end{equation}

We just keep dividing $n$ until we get an odd number. In this case we do the following:

\begin{equation}
	b^n = b\,b^{n-1} \; \text{and} \; a\,b^n = a\,b\,b^{n-1} = a_{\text{new}}\,b^{n_{\text{new}}}
\end{equation}

From here it's clear that b goes to a and the quantity remains intact.

In the end of the process we will be left with $n=1$ and the equation will look like this:

\begin{equation}
	a\,b^1 = a\,b = a_{\text{new}}
\end{equation}

We can see that the answer is given by the value of a at the end of the process.
